simple

src/Assembly/BoundedWord.v
@@ -14,20 +14,30 @@ Section BoundedWord.
 
   (* Word Operations *)
 
-  Definition wshiftr (w: word n) (bits: nat): word n.
+  Definition shiftr (w: word n) (bits: nat): word n.
     destruct (le_dec bits n).
 
     - replace n with (bits + (n - bits)) in * by (abstract intuition).
       refine (zext (split1 bits (n - bits) w) (n - bits)).
 
-    - exact w.
-
+    - exact (wzero n).
   Defined.
 
-  Lemma wshiftr_spec: forall (w : word n) (bits: nat),
-      wordToN (wshiftr w n) = N.shiftr (wordToN w) (N.of_nat n).
-    intros.
-    admit.
+  Lemma shiftr_spec: forall (w : word n) (bits: nat),
+      wordToN (shiftr w bits) = N.shiftr (wordToN w) (N.of_nat bits).
+    intros; unfold shiftr; destruct (le_dec bits n).
+
+    - admit.
+
+    - replace (wordToN (wzero n)) with 0%N by admit.
+      unfold N.shiftr.
+      induction bits.
+
+      + replace (N.of_nat 0) with 0%N by intuition.
+        assert (n = 0) by intuition; clear n0; subst.
+        replace w with WO; intuition.
+
+      + induction bits; admit.
   Qed.
 
   Definition mask (m: nat) (w: word n): word n.
@@ -37,10 +47,9 @@ Section BoundedWord.
       refine (w ^& (zext (wones m) (n - m))).
 
     - exact w.
-
   Defined.
 
-  (* First, we make our BoundedWord sigma type *)
+  (* Definitions of Inequality and simple bounds. *)
   Definition wordLeN {n: nat} (a: word n) (b: N): Prop :=
     (wordToN a <= b)%N.
 
@@ -71,6 +80,26 @@ Section BoundedWord.
   Ltac preomega := unfold wordLeN; intros; ge_to_le; pre_nomega.
 
   Hint Rewrite wordToN_nat Nat2N.inj_add N2Nat.inj_add Nat2N.inj_mul N2Nat.inj_mul Npow2_nat : N.
+
+  Theorem word_size_bound : forall (w: word n),
+    w <= Npow2 n - 1.
+  Proof.
+    intros; unfold wordLeN; rewrite wordToN_nat.
+
+    assert (B := wordToNat_bound w);
+      rewrite <- Npow2_nat in B;
+      apply nat_compare_lt in B.
+
+    unfold N.le; intuition;
+      rewrite N2Nat.inj_compare in H;
+      rewrite Nat2N.id in H.
+
+    apply nat_compare_lt in B.
+    apply nat_compare_gt in H.
+
+    replace (N.to_nat (Npow2 n)) with (S (N.to_nat (Npow2 n - 1))) in * by admit.
+    intuition.
+  Qed.
 
   Theorem constant_bound_N : forall k,
     NToWord n k <= k.
@@ -131,24 +160,41 @@ Section BoundedWord.
     apply Mult.mult_le_compat; nomega.
   Qed.
 
-  Theorem shiftr_bound : forall (w1 w2 : word n) b1 b2,
-    w1 <= b1
-    -> w2 <= b2
-    -> w1 ^* w2 <= b1 * b2.
+  Theorem shiftr_bound : forall (w : word n) b bits,
+    w <= b
+    -> shiftr w bits <= N.shiftr b (N.of_nat bits).
   Proof.
+    admit.
   Qed.
 
-  Theorem mask_bound : forall (w1 w2 : word n) b1 b2 a b,
-    w1 <= b1
-    -> w2 <= b2
-    -> word (a + b) = word (n)
-    -> w1 ^& zext (wones a) b <= zext (wones a) b.
+  Theorem mask_bound : forall (w : word n) m,
+    mask m w <= Npow2 m - 1.
   Proof.
+    admit.
+  Qed.
+
+  Theorem mask_update_bound : forall (w : word n) b m,
+    w <= b
+    -> mask m w <= (N.min b (Npow2 m - 1)).
+  Proof.
+    admit.
   Qed.
 
 
-  Ltac word_bound := repeat (eassumption || apply wplus_bound || apply wmult_bound
-                             || apply constant_bound_N || apply constant_bound_nat).
+  Ltac word_bound :=
+    repeat (
+       eassumption
+       || apply wplus_bound
+       || apply wmult_bound
+       || apply mask_update_bound
+       || apply mask_bound
+       || apply shiftr_bound
+       || apply constant_bound_N
+       || apply constant_bound_nat
+       || apply word_size_bound
+      ).
+
+  Notation "$" := (natToWord _).
 
   Lemma example1 : forall (w1 w2 w3 w4 : word n) b1 b2 b3 b4,
     w1 <= b1
@@ -161,11 +207,9 @@ Section BoundedWord.
     word_bound.
   Defined.
 
-  Eval simpl in fun (w1 w2 w3 w4 : word n) (b1 b2 b3 b4 : N)
+  (* Eval simpl in fun (w1 w2 w3 w4 : word n) (b1 b2 b3 b4 : N)
                     (H1 : w1 <= b1) (H2 : w2 <= b2) (H3 : w3 <= b3) (H4 : w4 <= b4) =>
-                  projT1 (example1 H1 H2 H3 H4).
-
-  Notation "$" := (natToWord _).
+                  projT1 (example1 H1 H2 H3 H4). *)
 
   Lemma example2 : forall (w1 w2 w3 w4 : word n) b1 b2 b3 b4,
     w1 <= b1
@@ -178,9 +222,9 @@ Section BoundedWord.
     word_bound.
   Defined.
 
-  Eval simpl in fun (w1 w2 w3 w4 : word n) (b1 b2 b3 b4 : N)
+  (*Eval simpl in fun (w1 w2 w3 w4 : word n) (b1 b2 b3 b4 : N)
                     (H1 : w1 <= b1) (H2 : w2 <= b2) (H3 : w3 <= b3) (H4 : w4 <= b4) =>
-                  projT1 (example2 H1 H2 H3 H4).
+                  projT1 (example2 H1 H2 H3 H4). *)
 
   Lemma example3 : forall (w1 w2 w3 w4 : word n),
     w1 <= Npow2 3
@@ -193,130 +237,165 @@ Section BoundedWord.
     word_bound.
   Defined.
 
-  Eval simpl in fun (w1 w2 w3 w4 : word n)
+  (* Eval simpl in fun (w1 w2 w3 w4 : word n)
                     (H1 : w1 <= _) (H2 : w2 <= _) (H3 : w3 <= _) (H4 : w4 <= _) =>
-                  projT1 (example3 H1 H2 H3 H4).
+                  projT1 (example3 H1 H2 H3 H4). *)
 
+End BoundedWord.
 
-  Section MulmodExamples.
+Section MulmodExamples.
 
-    Lemma example_and : forall x : word 32, wand x (NToWord 32 (N.ones 10)) <= 1023.
-    Abort.
+  Notation "A <= B" := (wordLeN A B) (at level 70).
+  Notation "$" := (natToWord _).
+
+  Ltac word_bound :=
+    repeat (
+       eassumption
+       || apply (wplus_bound 32)
+       || apply (wmult_bound 32)
+       || apply (mask_update_bound 32)
+       || apply (mask_bound 32)
+       || apply (shiftr_bound 32)
+       || apply (constant_bound_N 32)
+       || apply (constant_bound_nat 32)
+       || apply (word_size_bound 32)
+      ).
+
+  Lemma example_and : forall x : word 32, wand x (NToWord 32 (N.ones 10)) <= 1023.
+    intros.
+    replace (wand x (NToWord 32 (N.ones 10))) with (mask 32 10 x) by admit.
+    word_bound.
+  Qed.
     
-    Variable shiftrl : forall {l}, word l -> nat -> word l. (* "logical" aka "unsigned" bitshift *)
-    Hypothesis shiftrl_spec : forall {l} (w : word l) (n:nat), wordToN (shiftrl w n) = N.shiftr (wordToN w) (N.of_nat n).
+  Lemma example_shiftr : forall x : word 32, shiftr 32 x 30 <= 3.
+    intros.
+    replace 3%N with (N.shiftr (Npow2 32 - 1) (N.of_nat 30)) by (simpl; intuition).
 
-    Lemma example_shiftrl : forall x : word 32, shiftrl x 30 <= 3.
-    Abort.
+    (* word_bound works but it's slow *)
+    apply (shiftr_bound 32).
+    apply (word_size_bound 32).
+  Qed.
 
-    Lemma example_shiftrl2 : forall x : word 32, x <= 1023 -> shiftrl x 5 <= 31.
-    Abort.
+  Lemma example_shiftr2 : forall x : word 32, x <= 1023 -> shiftr 32 x 5 <= 31.
+    intros.
+    replace 31%N with (N.shiftr 1023%N 5%N) by (simpl; intuition).
+
+    (* word_bound works but it's slow *)
+    apply (shiftr_bound 32).
+    eassumption.
+  Qed.
     
-    Variable f0 f1 f2 f3 f4 f5 f6 f7 f8 f9 : word 32.
-    Variable g0 g1 g2 g3 g4 g5 g6 g7 g8 g9 : word 32.
-    Hypothesis Hf0 : f0 <= 2^26.
-    Hypothesis Hf1 : f1 <= 2^25.
-    Hypothesis Hf2 : f2 <= 2^26.
-    Hypothesis Hf3 : f3 <= 2^25.
-    Hypothesis Hf4 : f4 <= 2^26.
-    Hypothesis Hf5 : f5 <= 2^25.
-    Hypothesis Hf6 : f6 <= 2^26.
-    Hypothesis Hf7 : f7 <= 2^25.
-    Hypothesis Hf8 : f8 <= 2^26.
-    Hypothesis Hf9 : f9 <= 2^25.
-    Hypothesis Hg0 : g0 <= 2^26.
-    Hypothesis Hg1 : g1 <= 2^25.
-    Hypothesis Hg2 : g2 <= 2^26.
-    Hypothesis Hg3 : g3 <= 2^25.
-    Hypothesis Hg4 : g4 <= 2^26.
-    Hypothesis Hg5 : g5 <= 2^25.
-    Hypothesis Hg6 : g6 <= 2^26.
-    Hypothesis Hg7 : g7 <= 2^25.
-    Hypothesis Hg8 : g8 <= 2^26.
-    Hypothesis Hg9 : g9 <= 2^25.
+  Variable f0 f1 f2 f3 f4 f5 f6 f7 f8 f9 : word 32.
+  Variable g0 g1 g2 g3 g4 g5 g6 g7 g8 g9 : word 32.
+  Hypothesis Hf0 : f0 <= 2^26.
+  Hypothesis Hf1 : f1 <= 2^25.
+  Hypothesis Hf2 : f2 <= 2^26.
+  Hypothesis Hf3 : f3 <= 2^25.
+  Hypothesis Hf4 : f4 <= 2^26.
+  Hypothesis Hf5 : f5 <= 2^25.
+  Hypothesis Hf6 : f6 <= 2^26.
+  Hypothesis Hf7 : f7 <= 2^25.
+  Hypothesis Hf8 : f8 <= 2^26.
+  Hypothesis Hf9 : f9 <= 2^25.
+  Hypothesis Hg0 : g0 <= 2^26.
+  Hypothesis Hg1 : g1 <= 2^25.
+  Hypothesis Hg2 : g2 <= 2^26.
+  Hypothesis Hg3 : g3 <= 2^25.
+  Hypothesis Hg4 : g4 <= 2^26.
+  Hypothesis Hg5 : g5 <= 2^25.
+  Hypothesis Hg6 : g6 <= 2^26.
+  Hypothesis Hg7 : g7 <= 2^25.
+  Hypothesis Hg8 : g8 <= 2^26.
+  Hypothesis Hg9 : g9 <= 2^25.
     
-    Lemma example_mulmod_s_ppt : { b | f0 ^* g0  <= b}.
-    Abort.
+  Lemma example_mulmod_s_ppt : { b | f0 ^* g0  <= b}.
+    eexists.
+    word_bound.
+  Defined.
 
-    Lemma example_mulmod_s_pp :  { b | f0 ^* g0 ^+  $19 ^* (f9 ^* g1 ^* $2 ^+ f8 ^* g2 ^+ f7 ^* g3 ^* $2 ^+ f6 ^* g4 ^+ f5 ^* g5 ^* $2 ^+ f4 ^* g6 ^+ f3 ^* g7 ^* $2 ^+ f2 ^* g8 ^+  f1 ^* g9 ^* $2) <= b}.
-    Abort.
+  Lemma example_mulmod_s_pp :  { b | f0 ^* g0 ^+ $19 ^* (f9 ^* g1 ^* $2 ^+ f8 ^* g2 ^+ f7 ^* g3 ^* $2 ^+ f6 ^* g4 ^+ f5 ^* g5 ^* $2 ^+ f4 ^* g6 ^+ f3 ^* g7 ^* $2 ^+ f2 ^* g8 ^+  f1 ^* g9 ^* $2) <= b}.
+    eexists.
+    word_bound.
+  Defined.
 
-    Lemma example_mulmod_s_pp_shiftrl :
-        { b | shiftrl (f0 ^* g0 ^+  $19 ^* (f9 ^* g1 ^* $2 ^+ f8 ^* g2 ^+ f7 ^* g3 ^* $2 ^+ f6 ^* g4 ^+ f5 ^* g5 ^* $2 ^+ f4 ^* g6 ^+ f3 ^* g7 ^* $2 ^+ f2 ^* g8 ^+  f1 ^* g9 ^* $2)) 26 <= b}.
-    Abort.
+  Lemma example_mulmod_s_pp_shiftr :
+      { b | shiftr (f0 ^* g0 ^+  $19 ^* (f9 ^* g1 ^* $2 ^+ f8 ^* g2 ^+ f7 ^* g3 ^* $2 ^+ f6 ^* g4 ^+ f5 ^* g5 ^* $2 ^+ f4 ^* g6 ^+ f3 ^* g7 ^* $2 ^+ f2 ^* g8 ^+  f1 ^* g9 ^* $2)) 26 <= b}.
+    eexists.
+    word_bound.
+  Qed.
 
-    Lemma example_mulmod_u_fg1 :  { b |
-          (let y : word 32 := (* the type declarations on the let-s make type inference not take forever *)
-             (f0 ^* g0 ^+
-              $19 ^*
-              (f9 ^* g1 ^* $2 ^+ f8 ^* g2 ^+ f7 ^* g3 ^* $2 ^+ f6 ^* g4 ^+ f5 ^* g5 ^* $2 ^+ f4 ^* g6 ^+ f3 ^* g7 ^* $2 ^+ f2 ^* g8 ^+
-               f1 ^* g9 ^* $2)) in
-           let y0 : word 32 :=
-             (shiftrl y 26 ^+
-              (f1 ^* g0 ^+ f0 ^* g1 ^+
-               $19 ^* (f9 ^* g2 ^+ f8 ^* g3 ^+ f7 ^* g4 ^+ f6 ^* g5 ^+ f5 ^* g6 ^+ f4 ^* g7 ^+ f3 ^* g8 ^+ f2 ^* g9))) in
-           let y1 : word 32 :=
-             (shiftrl y0 25 ^+
-              (f2 ^* g0 ^+ f1 ^* g1 ^* $2 ^+ f0 ^* g2 ^+
-               $19 ^* (f9 ^* g3 ^* $2 ^+ f8 ^* g4 ^+ f7 ^* g5 ^* $2 ^+ f6 ^* g6 ^+ f5 ^* g7 ^* $2 ^+ f4 ^* g8 ^+ f3 ^* g9 ^* $2))) in
-           let y2 : word 32 :=
-             (shiftrl y1 26 ^+
-              (f3 ^* g0 ^+ f2 ^* g1 ^+ f1 ^* g2 ^+ f0 ^* g3 ^+
-               $19 ^* (f9 ^* g4 ^+ f8 ^* g5 ^+ f7 ^* g6 ^+ f6 ^* g7 ^+ f5 ^* g8 ^+ f4 ^* g9))) in
-           let y3 : word 32 :=
-             (shiftrl y2 25 ^+
-              (f4 ^* g0 ^+ f3 ^* g1 ^* $2 ^+ f2 ^* g2 ^+ f1 ^* g3 ^* $2 ^+ f0 ^* g4 ^+
-               $19 ^* (f9 ^* g5 ^* $2 ^+ f8 ^* g6 ^+ f7 ^* g7 ^* $2 ^+ f6 ^* g8 ^+ f5 ^* g9 ^* $2))) in
-           let y4 : word 32 :=
-             (shiftrl y3 26 ^+
-              (f5 ^* g0 ^+ f4 ^* g1 ^+ f3 ^* g2 ^+ f2 ^* g3 ^+ f1 ^* g4 ^+ f0 ^* g5 ^+
-               $19 ^* (f9 ^* g6 ^+ f8 ^* g7 ^+ f7 ^* g8 ^+ f6 ^* g9))) in
-           let y5 : word 32 :=
-             (shiftrl y4 25 ^+
-              (f6 ^* g0 ^+ f5 ^* g1 ^* $2 ^+ f4 ^* g2 ^+ f3 ^* g3 ^* $2 ^+ f2 ^* g4 ^+ f1 ^* g5 ^* $2 ^+ f0 ^* g6 ^+
-               $19 ^* (f9 ^* g7 ^* $2 ^+ f8 ^* g8 ^+ f7 ^* g9 ^* $2))) in
-           let y6 : word 32 :=
-             (shiftrl y5 26 ^+
-              (f7 ^* g0 ^+ f6 ^* g1 ^+ f5 ^* g2 ^+ f4 ^* g3 ^+ f3 ^* g4 ^+ f2 ^* g5 ^+ f1 ^* g6 ^+ f0 ^* g7 ^+
-               $19 ^* (f9 ^* g8 ^+ f8 ^* g9))) in
-           let y7 : word 32 :=
-             (shiftrl y6 25 ^+
-              (f8 ^* g0 ^+ f7 ^* g1 ^* $2 ^+ f6 ^* g2 ^+ f5 ^* g3 ^* $2 ^+ f4 ^* g4 ^+ f3 ^* g5 ^* $2 ^+ f2 ^* g6 ^+ f1 ^* g7 ^* $2 ^+
-               f0 ^* g8 ^+ $19 ^* f9 ^* g9 ^* $2)) in
-           let y8 : word 32 :=
-             (shiftrl y7 26 ^+
-              (f9 ^* g0 ^+ f8 ^* g1 ^+ f7 ^* g2 ^+ f6 ^* g3 ^+ f5 ^* g4 ^+ f4 ^* g5 ^+ f3 ^* g6 ^+ f2 ^* g7 ^+ f1 ^* g8 ^+
-               f0 ^* g9)) in
-           let y9 : word 32 :=
-             ($19 ^* shiftrl y8 25 ^+
-              wand
-                (f0 ^* g0 ^+
-                 $19 ^*
-                 (f9 ^* g1 ^* $2 ^+ f8 ^* g2 ^+ f7 ^* g3 ^* $2 ^+ f6 ^* g4 ^+ f5 ^* g5 ^* $2 ^+ f4 ^* g6 ^+ f3 ^* g7 ^* $2 ^+
-                  f2 ^* g8 ^+ f1 ^* g9 ^* $2)) (@NToWord 32 (N.ones 26%N))) in
-           let fg1 : word 32 := (shiftrl y9 26 ^+
+  Lemma example_mulmod_u_fg1 :  { b |
+        (let y : word 32 := (* the type declarations on the let-s make type inference not take forever *)
+           (f0 ^* g0 ^+
+            $19 ^*
+            (f9 ^* g1 ^* $2 ^+ f8 ^* g2 ^+ f7 ^* g3 ^* $2 ^+ f6 ^* g4 ^+ f5 ^* g5 ^* $2 ^+ f4 ^* g6 ^+ f3 ^* g7 ^* $2 ^+ f2 ^* g8 ^+
+             f1 ^* g9 ^* $2)) in
+         let y0 : word 32 :=
+           (shiftr y 26 ^+
+            (f1 ^* g0 ^+ f0 ^* g1 ^+
+             $19 ^* (f9 ^* g2 ^+ f8 ^* g3 ^+ f7 ^* g4 ^+ f6 ^* g5 ^+ f5 ^* g6 ^+ f4 ^* g7 ^+ f3 ^* g8 ^+ f2 ^* g9))) in
+         let y1 : word 32 :=
+           (shiftr y0 25 ^+
+            (f2 ^* g0 ^+ f1 ^* g1 ^* $2 ^+ f0 ^* g2 ^+
+             $19 ^* (f9 ^* g3 ^* $2 ^+ f8 ^* g4 ^+ f7 ^* g5 ^* $2 ^+ f6 ^* g6 ^+ f5 ^* g7 ^* $2 ^+ f4 ^* g8 ^+ f3 ^* g9 ^* $2))) in
+         let y2 : word 32 :=
+           (shiftr y1 26 ^+
+            (f3 ^* g0 ^+ f2 ^* g1 ^+ f1 ^* g2 ^+ f0 ^* g3 ^+
+             $19 ^* (f9 ^* g4 ^+ f8 ^* g5 ^+ f7 ^* g6 ^+ f6 ^* g7 ^+ f5 ^* g8 ^+ f4 ^* g9))) in
+         let y3 : word 32 :=
+           (shiftr y2 25 ^+
+            (f4 ^* g0 ^+ f3 ^* g1 ^* $2 ^+ f2 ^* g2 ^+ f1 ^* g3 ^* $2 ^+ f0 ^* g4 ^+
+             $19 ^* (f9 ^* g5 ^* $2 ^+ f8 ^* g6 ^+ f7 ^* g7 ^* $2 ^+ f6 ^* g8 ^+ f5 ^* g9 ^* $2))) in
+         let y4 : word 32 :=
+           (shiftr y3 26 ^+
+            (f5 ^* g0 ^+ f4 ^* g1 ^+ f3 ^* g2 ^+ f2 ^* g3 ^+ f1 ^* g4 ^+ f0 ^* g5 ^+
+             $19 ^* (f9 ^* g6 ^+ f8 ^* g7 ^+ f7 ^* g8 ^+ f6 ^* g9))) in
+         let y5 : word 32 :=
+           (shiftr y4 25 ^+
+            (f6 ^* g0 ^+ f5 ^* g1 ^* $2 ^+ f4 ^* g2 ^+ f3 ^* g3 ^* $2 ^+ f2 ^* g4 ^+ f1 ^* g5 ^* $2 ^+ f0 ^* g6 ^+
+             $19 ^* (f9 ^* g7 ^* $2 ^+ f8 ^* g8 ^+ f7 ^* g9 ^* $2))) in
+         let y6 : word 32 :=
+           (shiftr y5 26 ^+
+            (f7 ^* g0 ^+ f6 ^* g1 ^+ f5 ^* g2 ^+ f4 ^* g3 ^+ f3 ^* g4 ^+ f2 ^* g5 ^+ f1 ^* g6 ^+ f0 ^* g7 ^+
+             $19 ^* (f9 ^* g8 ^+ f8 ^* g9))) in
+         let y7 : word 32 :=
+           (shiftr y6 25 ^+
+            (f8 ^* g0 ^+ f7 ^* g1 ^* $2 ^+ f6 ^* g2 ^+ f5 ^* g3 ^* $2 ^+ f4 ^* g4 ^+ f3 ^* g5 ^* $2 ^+ f2 ^* g6 ^+ f1 ^* g7 ^* $2 ^+
+             f0 ^* g8 ^+ $19 ^* f9 ^* g9 ^* $2)) in
+         let y8 : word 32 :=
+           (shiftr y7 26 ^+
+            (f9 ^* g0 ^+ f8 ^* g1 ^+ f7 ^* g2 ^+ f6 ^* g3 ^+ f5 ^* g4 ^+ f4 ^* g5 ^+ f3 ^* g6 ^+ f2 ^* g7 ^+ f1 ^* g8 ^+
+             f0 ^* g9)) in
+         let y9 : word 32 :=
+           ($19 ^* shiftr y8 25 ^+
             wand
-              (shiftrl y 26 ^+
-               (f1 ^* g0 ^+ f0 ^* g1 ^+
-                $19 ^* (f9 ^* g2 ^+ f8 ^* g3 ^+ f7 ^* g4 ^+ f6 ^* g5 ^+ f5 ^* g6 ^+ f4 ^* g7 ^+ f3 ^* g8 ^+ f2 ^* g9)))
-              (@NToWord 32 (N.ones 26%N))) in
-           fg1) <= b }.
-    Abort.
+              (f0 ^* g0 ^+
+               $19 ^*
+               (f9 ^* g1 ^* $2 ^+ f8 ^* g2 ^+ f7 ^* g3 ^* $2 ^+ f6 ^* g4 ^+ f5 ^* g5 ^* $2 ^+ f4 ^* g6 ^+ f3 ^* g7 ^* $2 ^+
+                f2 ^* g8 ^+ f1 ^* g9 ^* $2)) (@NToWord 32 (N.ones 26%N))) in
+         let fg1 : word 32 := (shiftr y9 26 ^+
+          wand
+            (shiftr y 26 ^+
+             (f1 ^* g0 ^+ f0 ^* g1 ^+
+              $19 ^* (f9 ^* g2 ^+ f8 ^* g3 ^+ f7 ^* g4 ^+ f6 ^* g5 ^+ f5 ^* g6 ^+ f4 ^* g7 ^+ f3 ^* g8 ^+ f2 ^* g9)))
+            (@NToWord 32 (N.ones 26%N))) in
+         fg1) <= b }.
+  Abort.
 
-    Require Import ZArith.
-    Variable shiftra : forall {l}, word l -> nat -> word l. (* "arithmetic" aka "signed" bitshift *)
-    Hypothesis shiftra_spec : forall {l} (w : word l) (n:nat), wordToZ (shiftra w n) = Z.shiftr (wordToZ w) (Z.of_nat n).
+  Require Import ZArith.
+  Variable shiftra : forall {l}, word l -> nat -> word l. (* "arithmetic" aka "signed" bitshift *)
+  Hypothesis shiftra_spec : forall {l} (w : word l) (n:nat), wordToZ (shiftra w n) = Z.shiftr (wordToZ w) (Z.of_nat n).
 
-    Lemma example_shiftra : forall x : word 4, shiftra x 2 <= 15.
-    Abort.
+  Lemma example_shiftra : forall x : word 4, shiftra x 2 <= 15.
+  Abort.
 
-    Lemma example_shiftra : forall x : word 4, x <= 7 -> shiftra x 2 <= 1.
-    Abort.
+  Lemma example_shiftra : forall x : word 4, x <= 7 -> shiftra x 2 <= 1.
+  Abort.
 
-    Lemma example_mulmod_s_pp_shiftra :
-        { b | shiftra (f0 ^* g0 ^+  $19 ^* (f9 ^* g1 ^* $2 ^+ f8 ^* g2 ^+ f7 ^* g3 ^* $2 ^+ f6 ^* g4 ^+ f5 ^* g5 ^* $2 ^+ f4 ^* g6 ^+ f3 ^* g7 ^* $2 ^+ f2 ^* g8 ^+  f1 ^* g9 ^* $2)) 26 <= b}.
-    Abort.
-  End MulmodExamples.
+  Lemma example_mulmod_s_pp_shiftra :
+      { b | shiftra (f0 ^* g0 ^+  $19 ^* (f9 ^* g1 ^* $2 ^+ f8 ^* g2 ^+ f7 ^* g3 ^* $2 ^+ f6 ^* g4 ^+ f5 ^* g5 ^* $2 ^+ f4 ^* g6 ^+ f3 ^* g7 ^* $2 ^+ f2 ^* g8 ^+  f1 ^* g9 ^* $2)) 26 <= b}.
+  Abort.
+End MulmodExamples.
 
 (* Old lemmas that might end up being useful
 
@@ -530,5 +609,3 @@ Section BoundedWord.
     unfold_ops; simpl.
     match_match; word_simpl.
   Qed. *)
-
-End BoundedWord.
